LeanSAT/Reflect/BVExpr/BitBlast/Lemmas/RotateRight.lean
@@ -11,7 +11,7 @@ open AIG
 namespace BVExpr
 namespace bitblast
 
-variable [BEq α] [Hashable α] [DecidableEq α]
+variable [Hashable α] [DecidableEq α]
 
 namespace blastRotateRight
 
